add iAuIntro tactic to prove an atomic update; introduce atomic_step

theories/bi/lib/atomic.v
@@ -1,30 +1,30 @@
 From iris.bi Require Export bi updates.
 From iris.bi.lib Require Import fixpoint laterable.
 From stdpp Require Import coPset.
-From iris.proofmode Require Import tactics.
+From iris.proofmode Require Import coq_tactics tactics.
 Set Default Proof Using "Type".
 
-(** atomic_update as a fixed-point of the equation
-   AU = ∃ P. ▷ P ∗ □ (▷ P ==∗ α ∗ (α ==∗ AU) ∧ (β ==∗ Q))
- *)
 Section definition.
-  Context `{BiFUpd PROP} {A B : Type}
-    (α : A → PROP) (* atomic pre-condition *)
-    (β : A → B → PROP) (* atomic post-condition *)
+  Context `{BiFUpd PROP} {A B : Type}.
+  Implicit Types
     (Eo Em : coPset) (* outside/module masks *)
+    (α : A → PROP) (* atomic pre-condition *)
+    (P : PROP) (* abortion condition *)
+    (β : A → B → PROP) (* atomic post-condition *)
     (Φ : A → B → PROP) (* post-condition *)
   .
 
-  Definition atomic_shift (P P' : PROP) : PROP :=
-    (□ (∀ E, ⌜Eo ⊆ E⌝ → P ={E, E∖Em}=∗ ∃ x, α x ∗
-          ((α x ={E∖Em, E}=∗ P') ∧ (∀ y, β x y ={E∖Em, E}=∗ Φ x y)))
+(** atomic_step as the "introduction form" of atomic updates *)
+  Definition atomic_step Eo Em α P β Φ : PROP :=
+    (|={Eo, Eo∖Em}=> ∃ x, α x ∗
+          ((α x ={Eo∖Em, Eo}=∗ P) ∧ (∀ y, β x y ={Eo∖Em, Eo}=∗ Φ x y))
     )%I.
 
-  Lemma atomic_shift_mono P P1 P2:
-    □ (P1 -∗ P2) -∗ □ (atomic_shift P P1 -∗ atomic_shift P P2).
+  Lemma atomic_shift_mono Eo Em α P1 P2 β Φ :
+    □ (P1 -∗ P2) -∗
+    □ (atomic_step Eo Em α P1 β Φ -∗ atomic_step Eo Em α P2 β Φ).
   Proof.
-    iIntros "#HP12 !# #AS !# * % HP".
-    iMod ("AS" with "[% //] HP") as (x) "[Hα Hclose]".
+    iIntros "#HP12 !# AS". iMod "AS" as (x) "[Hα Hclose]".
     iModIntro. iExists x. iFrame "Hα". iSplit.
     - iIntros "Hα". iDestruct "Hclose" as "[Hclose _]".
       iApply "HP12". iApply "Hclose". done.
@@ -32,21 +32,28 @@ Section definition.
       iApply "Hclose". done.
   Qed.
 
+(** atomic_update as a fixed-point of the equation
+   AU = ∃ P. ▷ P ∗ □ (▷ P ==∗ α ∗ (α ==∗ AU) ∧ (β ==∗ Q))
+ *)
+  Context Eo Em α β Φ.
+
   Definition atomic_update_pre (Ψ : () → PROP) (_ : ()) : PROP :=
-    (∃ (P : PROP), ▷ P ∗ atomic_shift (▷ P) (Ψ ()))%I.
+    (∃ (P : PROP), ▷ P ∗
+     □ (∀ E, ⌜Eo ⊆ E⌝ → (▷ P) -∗ atomic_step E Em α (Ψ ()) β Φ))%I.
 
   Local Instance atomic_update_pre_mono : BiMonoPred atomic_update_pre.
   Proof.
     constructor.
     - iIntros (P1 P2) "#HP12". iIntros ([]) "AU".
-      iDestruct "AU" as (P) "[HP AS]". iExists P. iFrame.
-      iApply (atomic_shift_mono with "[HP12]"); last done.
-      iAlways. iApply "HP12".
+      iDestruct "AU" as (P) "[HP #AS]". iExists P. iFrame.
+      iIntros "!# * % HP". iApply (atomic_shift_mono with "HP12").
+      iApply ("AS" with "[%]"); done.
     - intros ??. solve_proper.
   Qed.
 
   Definition atomic_update_def :=
     bi_greatest_fixpoint atomic_update_pre ().
+
 End definition.
 
 (** Seal it *)
@@ -62,13 +69,32 @@ Section lemmas.
 
   Local Existing Instance atomic_update_pre_mono.
 
+  Global Instance atomic_step_ne Eo Em n :
+    Proper (
+        pointwise_relation A (dist n) ==>
+        dist n ==>
+        pointwise_relation A (pointwise_relation B (dist n)) ==>
+        pointwise_relation A (pointwise_relation B (dist n)) ==>
+        dist n
+    ) (atomic_step (PROP:=PROP) Eo Em).
+  Proof. solve_proper. Qed.
+
+  Global Instance atomic_update_ne Eo Em n :
+    Proper (
+        pointwise_relation A (dist n) ==>
+        pointwise_relation A (pointwise_relation B (dist n)) ==>
+        pointwise_relation A (pointwise_relation B (dist n)) ==>
+        dist n
+    ) (atomic_update (PROP:=PROP) Eo Em).
+  Proof.
+    rewrite atomic_update_eq /atomic_update_def /atomic_update_pre. solve_proper.
+  Qed.
+
   (** The ellimination form: an accessor *)
-  Lemma aupd_acc α β Eo Em Φ E :
+  Lemma aupd_acc  Eo Em E α β Φ :
     Eo ⊆ E →
-    atomic_update α β Eo Em Φ -∗
-    |={E, E∖Em}=> ∃ x, α x ∗
-      ((α x ={E∖Em, E}=∗ atomic_update α β Eo Em Φ) ∧
-       (∀ y, β x y ={E∖Em, E}=∗ Φ x y)).
+    atomic_update Eo Em α β Φ -∗
+    atomic_step E Em α (atomic_update Eo Em α β Φ) β Φ.
   Proof using Type*.
     rewrite atomic_update_eq {1}/atomic_update_def /=. iIntros (HE) "HUpd".
     iPoseProof (greatest_fixpoint_unfold_1 with "HUpd") as "HUpd".
@@ -77,8 +103,8 @@ Section lemmas.
     iModIntro. iExists x. iFrame.
   Qed.
 
-  Global Instance aupd_laterable α β Eo Em Φ :
-    Laterable (atomic_update α β Eo Em Φ).
+  Global Instance aupd_laterable Eo Em α β Φ :
+    Laterable (atomic_update Eo Em α β Φ).
   Proof.
     rewrite /Laterable atomic_update_eq {1}/atomic_update_def /=. iIntros "AU".
     iPoseProof (greatest_fixpoint_unfold_1 with "AU") as (P) "[HP #AS]".
@@ -86,20 +112,18 @@ Section lemmas.
     iApply greatest_fixpoint_unfold_2. iExists P. iFrame "#∗".
   Qed.
 
-  Lemma aupd_intro P α β Eo Em Φ :
-    Em ⊆ Eo → Laterable P →
-    P -∗
-    □ (P -∗ |={Eo, Eo∖Em}=> ∃ x, α x ∗
-      ((α x ={Eo∖Em, Eo}=∗ P) ∧ (∀ y, β x y ={Eo∖Em, Eo}=∗ Φ x y))) -∗
-    atomic_update α β Eo Em Φ.
+  Lemma aupd_intro P Q α β Eo Em Φ :
+    Em ⊆ Eo → Affine P → Persistent P → Laterable Q →
+    (P ∗ Q -∗ atomic_step Eo Em α Q β Φ) →
+    P ∗ Q -∗ atomic_update Eo Em α β Φ.
   Proof.
     rewrite atomic_update_eq {1}/atomic_update_def /=.
-    iIntros (??) "HP #AU".
-    iApply (greatest_fixpoint_coind _ (λ _, P)); last done. iIntros "!#" ([]) "HP".
-    iDestruct (laterable with "HP") as (P') "[HP' #HPi]". iExists P'. iFrame.
-    iIntros "!#" (E HE) "HP'". iDestruct ("HPi" with "HP'") as ">HP {HPi}".
+    iIntros (???? HAU) "[#HP HQ]".
+    iApply (greatest_fixpoint_coind _ (λ _, Q)); last done. iIntros "!#" ([]) "HQ".
+    iDestruct (laterable with "HQ") as (Q') "[HQ' #HQi]". iExists Q'. iFrame.
+    iIntros "!#" (E HE) "HQ'". iDestruct ("HQi" with "HQ'") as ">HQ {HQi}".
     iApply fupd_mask_frame_diff_open; last
-      iMod ("AU" with "HP") as (x) "[Hα Hclose] {AU}"; [done..|].
+      iMod (HAU with "[$HQ]") as (x) "[Hα Hclose]"; [done..|].
     iModIntro. iExists x. iFrame. iSplit.
     - iDestruct "Hclose" as "[Hclose _]". iIntros "Hα".
       iApply fupd_mask_frame_diff_close; last (by iApply "Hclose"); done.
@@ -107,3 +131,33 @@ Section lemmas.
       iApply fupd_mask_frame_diff_close; last (by iApply "Hclose"); done.
   Qed.
 End lemmas.
+
+(** ProofMode support for atomic updates *)
+
+Section proof_mode.
+  Context `{BiFUpd PROP} {A B : Type}.
+  Implicit Types (α : A → PROP) (β: A → B → PROP) (P : PROP) (Φ : A → B → PROP).
+
+  Lemma tac_aupd_intro Γp Γs n α β Eo Em Φ P :
+    Em ⊆ Eo →
+    Timeless (PROP:=PROP) emp →
+    TCForall Laterable (env_to_list Γs) →
+    P = prop_of_env Γs →
+    envs_entails (Envs Γp Γs n) (atomic_step Eo Em α P β Φ) →
+    envs_entails (Envs Γp Γs n) (atomic_update Eo Em α β Φ).
+  Proof.
+    intros ?? HΓs ->. rewrite envs_entails_eq of_envs_eq' /atomic_step /=.
+    setoid_rewrite prop_of_env_sound =>HAU.
+    apply aupd_intro; [done|apply _..|]. done.
+  Qed. 
+End proof_mode.
+
+(** Now the coq-level tactics *)
+
+Tactic Notation "iAuIntro" :=
+  iStartProof; eapply tac_aupd_intro; [
+    (* Em ⊆ Eo: to be proven by user *)
+  | iSolveTC || fail "iAuIntro: emp is not timeless"
+  | iSolveTC || fail "Not all spatial assumptions are laterable"
+  | (* P = ...: make the P pretty *) env_reflexivity
+  | (* the new proof mode goal *) ].
