theories/heap_lang/lib/increment.v
@@ -21,23 +21,23 @@ Section increment.
 
   Lemma incr_spec (l: loc) :
         atomic_wp (incr #l)
+                  ⊤ ⊤
                   (λ (v: Z), aheap.(mapsto) l 1 #v)%I
                   (λ v (_:()), aheap.(mapsto) l 1 #(v + 1))%I
-                  ⊤ ⊤
                   (λ v _, #v).
   Proof.
     iIntros (Q Φ) "HQ AU". iLöb as "IH". wp_let.
-    wp_apply (load_spec with "HQ").
+    wp_apply (load_spec with "[HQ]"); first by iAccu.
     (* Prove the atomic shift for load *)
-    iApply (aupd_intro with "AU"); first done. iIntros "!# AU".
+    iAuIntro; first done.
     iMod (aupd_acc with "AU") as (x) "[H↦ [Hclose _]]"; first solve_ndisj.
     iModIntro. iExists (#x, 1%Qp). iFrame "H↦". iSplit; first done.
     iIntros ([]) "H↦". iMod ("Hclose" with "H↦") as "AU". iIntros "!> HQ".
     (* Now go on *)
     wp_let. wp_op. wp_bind (aheap.(cas) _)%I.
-    wp_apply (cas_spec with "HQ").
+    wp_apply (cas_spec with "[HQ]"); first by iAccu.
     (* Prove the atomic shift for CAS *)
-    iApply (aupd_intro with "AU"); first done. iIntros "!# AU".
+    iAuIntro; first done.
     iMod (aupd_acc with "AU") as (x') "[H↦ Hclose]"; first solve_ndisj.
     iModIntro. iExists #x'. iFrame. iSplit.
     { iDestruct "Hclose" as "[Hclose _]". iApply "Hclose". }
@@ -69,8 +69,7 @@ Section increment_client.
        to move this to the persisten context even without the additional □. *)
     iAssert (□ WP incr primitive_atomic_heap #l {{ _, True }})%I as "#Aupd".
     { iAlways. wp_apply (incr_spec with "[]"); first iEmpIntro. clear x.
-      iApply (aupd_intro with "[]"); try iEmpIntro; [done|apply _|]. iIntros "!# _".
-      iInv nroot as (x) ">H↦" "Hclose".
+      iAuIntro; first done. iInv nroot as (x) ">H↦" "Hclose".
       iMod fupd_intro_mask' as "Hclose2"; last iModIntro; first set_solver.
       iExists _. iFrame. iSplit.
       { iIntros "H↦". iMod "Hclose2" as "_". iMod ("Hclose" with "[-]"); last done.
