theories/program_logic/atomic.v
@@ -5,12 +5,12 @@ Set Default Proof Using "Type".
 
 Definition atomic_wp `{irisG Λ Σ} {A B : Type}
   (e: expr Λ) (* expression *)
+  (Eo Em : coPset) (* outside/module masks *)
   (α: A → iProp Σ) (* atomic pre-condition *)
   (β: A → B → iProp Σ) (* atomic post-condition *)
-  (Eo Em : coPset) (* outside/module masks *)
   (f: A → B → val Λ) (* Turn the return data into the return value *)
   : iProp Σ :=
-    (∀ Q Φ, Q -∗ atomic_update α β Eo Em (λ x y, Q -∗ Φ (f x y)) -∗
+    (∀ Q Φ, Q -∗ atomic_update Eo Em α β (λ x y, Q -∗ Φ (f x y)) -∗
              WP e {{ Φ }})%I.
 (* Note: To add a private postcondition, use
    atomic_update α β Eo Em (λ x y, POST x y -∗ Φ (f x y)) *)
